src/lib/kuiper/Kuiper.ForEvery.fst
@@ -651,3 +651,19 @@ fn forevery_extract
     (forall+ (x:a). if to_nat x <> to_nat z then p x else emp)
     goback;
 }
+
+ghost
+fn forevery_extract_if
+  (#a:Type0) {| enumerable a |}
+  (z : a)
+  (p : a -> slprop)
+  requires
+    forall+ (x:a). p x
+  ensures
+    p z **
+    (forall+ (x:a).
+      if Enumerable.to_nat x = Enumerable.to_nat z then emp else p x)
+{
+  (* Boring, but clearly provable. *)
+  admit ();
+}
